half of iak cert

keyCert.v
@@ -1,6 +1,394 @@
 Require Import Coq.Init.Nat.
 Require Import Coq.Sets.Ensembles.
 
+
+
+
+
+Inductive ak_val : Set :=
+| initial : ak_val
+| local : ak_val.
+
+Inductive ca_val : Set :=
+| tm : ca_val   (* tpm manufacturer *)
+| oem : ca_val  (* original equipment manufacturer *)
+| owner : ca_val.
+
+Inductive key_val : Set :=
+| EK : key_val              (* endorsement key *)
+| AK : ak_val -> key_val    (* attestation key *)
+| CA : ca_val -> key_val.   (* certificate authority key *)
+
+Inductive keyType : Type := 
+| Private : key_val -> keyType
+| Public : key_val -> keyType.
+
+(* TODO: nonce/secret *)
+(* TODO: id for tpm and device *)
+
+(* TODO: id : id_val -> message *)
+(* TODO: hash : message -> message *)
+(* TODO: credential : message -> secret -> message *)
+Inductive message : Type :=
+| key : keyType -> message
+| TPM2_Attest : keyType -> message
+| sign : message -> keyType -> message
+| credential : message -> message
+| encrypt : message -> keyType -> message
+| pair : message -> message -> message.
+
+(* TODO: MakeCert : keyType -> id*)
+(* TODO: TPM2_Hash : message -> command *)
+(* TODO: MakeCert : keyType -> id -> keyType -> command *)
+(* TODO: TPM2_MakeCredential : name -> secret -> keyType -> command *)
+(* TODO: CheckNonce *)
+Inductive command : Type :=
+| TPM2_Create : key_val -> command
+| TPM2_Certify : keyType -> keyType -> command
+| MakeCSR : message -> message -> keyType -> command
+| TPM2_Sign : message -> keyType -> command
+| CheckSig : message -> keyType -> command
+| TPM2_MakeCredential : keyType -> keyType -> command
+| TPM2_ActivateCredential : message -> keyType -> command
+| MakeCert : keyType -> keyType -> command
+| Sequence : command -> command -> command.
+
+Definition state := Ensemble message. (* ? should be decidable ? *)
+
+Notation "m1 , m2" := (pair m1 m2)  (at level 90, left associativity).
+Notation "c1 ; c2" := (Sequence c1 c2) (at level 90, left associativity).
+Notation "A : x" := (Add message A x) (at level 90, left associativity).
+
+Inductive execute : state -> command -> state -> Prop :=
+| E_Create : forall st v, 
+    execute st (TPM2_Create v) (st : (key (Private v)) : (key (Public v)))
+| E_Certify : forall st k k0,
+    In _ st (key k) ->
+    In _ st (key k0) ->
+    execute st (TPM2_Certify k k0) (st : (sign (TPM2_Attest k) k0))
+| E_MakeCSR : forall st m1 m2 k,
+    In _ st m1 ->
+    In _ st m2 ->
+    In _ st (key k) ->
+    execute st (MakeCSR m1 m2 k) (st : (m1, m2, (key k)))
+| E_Sign : forall st m k,
+    In _ st m ->
+    In _ st (key k) ->
+    execute st (TPM2_Sign m k) (st : (sign m k))
+| E_CheckSigAK : forall st m a,
+    In _ st (sign m (Private (AK a))) -> (* ? required ? *)
+    In _ st (key (Public (AK a))) ->
+    execute st (CheckSig (sign m (Private (AK a))) (Public (AK a))) st
+| E_CheckSigCA : forall st m c,
+    In _ st (sign m (Private (CA c))) -> (* ? required ? *)
+    In _ st (key (Public (CA c))) ->
+    execute st (CheckSig (sign m (Private (CA c))) (Public (CA c))) st
+| E_MakeCredential : forall st k k0, (* TODO: add secret credential *)
+    In _ st (key k) ->  (* TODO: replace with name *)
+    In _ st (key k0) ->
+    execute st (TPM2_MakeCredential k k0) (st : (encrypt (credential (key k)) k0))
+| E_ActivateCredential : forall st m,
+    In _ st (encrypt (credential m) (Private EK)) ->
+    In _ st (key (Public EK)) ->
+    (* TODO: add secret to state *)
+    execute st (TPM2_ActivateCredential (encrypt (credential m) (Private EK)) (Public EK)) (st : (credential m))
+| E_MakeCert : forall st k k0,
+    In _ st (key k) ->
+    In _ st (key k0) ->
+    execute st (MakeCert k k0) (st : (sign (key k) k0))
+| E_Sequence : forall st st' st'' c1 c2,
+    execute st c1 st' ->
+    execute st' c2 st'' ->
+    execute st (Sequence c1 c2) st''.
+
+
+
+
+
+
+
+Inductive discoverable : message -> state -> Prop :=
+| D_key : forall k,
+    discoverable (key k) (Singleton _ (key k))
+| D_Attest : forall k,
+    discoverable (TPM2_Attest k) (Singleton _ (TPM2_Attest k))
+| D_sign : forall m k st, 
+    discoverable m st ->
+    discoverable (sign m k) (st : (sign m k))
+| D_credential : forall m st,
+    discoverable m st ->
+    discoverable (credential m) (st : (credential m))
+| D_encrypt : forall m k,
+    discoverable (encrypt m k) (Singleton _ (encrypt m k))
+| D_pair : forall m1 m2 st1 st2,
+    discoverable m1 st1 ->
+    discoverable m2 st2 ->
+    discoverable (pair m1 m2) ((Union _ st1 st2) : (m1, m2)).
+    
+(* when sending a message the recipient can discover everything in this result *)
+Fixpoint send (m : message) : state :=
+match m with
+  | sign m0 k => (send m0) : (sign m0 k)
+  | credential m0 => (send m0) : (credential m0)
+  | pair m1 m2 => (Union _ (send m1) (send m2)) : (m1, m2)
+  | _ => Singleton _ m
+end.
+    
+Theorem discoverableSend : forall m st,
+discoverable m st ->
+send m = st.
+Proof.
+  intros m st H; induction H; simpl; subst; reflexivity.
+Qed.
+
+Lemma sendDiscoverable' : forall m,
+discoverable m (send m).
+Proof.
+  intros m; induction m; simpl; constructor; assumption.
+Qed.
+
+Theorem sendDiscoverable : forall m st,
+send m = st -> 
+discoverable m st.
+Proof.
+  intros m st H; induction m; subst; apply sendDiscoverable'.
+Qed.
+
+Theorem iff_DiscoverableSend : forall m st,
+discoverable m st <-> send m = st.
+Proof.
+  split.
+  - apply discoverableSend.
+  - apply sendDiscoverable.
+Qed.
+
+
+
+
+
+
+
+
+(* Owner creation of LAK certificate based on IAK certificate *)
+
+Definition ownerIni : state :=
+(*0*)(Singleton _ (key (Private (AK initial)))) :
+     (sign (key (Public (AK initial))) (Private (CA oem))).
+
+Definition lakCSR : message :=
+((sign (key (Public (AK initial))) (Private (CA oem))),
+ (sign (TPM2_Attest (Private (AK local))) (Private (AK initial))),
+ (key (Public (AK local)))).
+
+Definition ownerSteps : command :=
+(*1*)TPM2_Create (AK local) ;
+(*2*)TPM2_Certify (Private (AK local)) (Private (AK initial)) ;
+(*3*)MakeCSR (sign (key (Public (AK initial))) (Private (CA oem))) 
+             (sign (TPM2_Attest (Private (AK local))) (Private (AK initial))) 
+             (Public (AK local)) ;
+(*4*)TPM2_Sign lakCSR (Private (AK local)).
+
+Definition ownerFinal : state :=
+(*0*)ownerIni :
+(*1*)(key (Private (AK local))) :
+     (key (Public (AK local))) :
+(*2*)(sign (TPM2_Attest (Private (AK local))) (Private (AK initial))) :
+(*3*)lakCSR :
+(*4*)(sign lakCSR (Private (AK local))).
+
+(*
+Hint Unfold In ownerIni ownerSteps lakCSR ownerFinal: core.
+Hint Resolve Union_introl Union_intror In_singleton Extensionality_Ensembles: core.
+Hint Constructors execute : core.
+*)
+
+Theorem correct_ownerFinal :
+execute ownerIni ownerSteps ownerFinal.
+Proof.
+  unfold ownerFinal; unfold ownerIni; unfold ownerSteps; unfold lakCSR; simpl. 
+  repeat eapply E_Sequence. 
+  - apply E_Create.
+  - apply E_Certify. 
+  -- apply Union_introl. apply Union_intror. apply In_singleton.
+  -- apply Union_introl. apply Union_introl. apply Union_introl. apply In_singleton.
+  - apply E_MakeCSR.
+  -- apply Union_introl. apply Union_introl. apply Union_introl. apply Union_intror.
+     apply In_singleton.
+  -- apply Union_intror. apply In_singleton.
+  -- apply Union_introl. apply Union_intror. apply In_singleton.
+  - apply E_Sign.
+  -- apply Union_intror. apply In_singleton.
+  -- apply Union_introl. apply Union_introl. apply Union_introl. apply Union_intror.
+     apply In_singleton.
+Qed.
+
+(*5*)(* send 4 *)
+
+Definition caOwnerIni : state :=
+(*0*)(Singleton _ (key (Private (CA owner)))) :
+     (key (Public (CA oem))).
+
+Definition caOwnerSteps : command :=
+(*6*)(CheckSig (sign lakCSR (Private (AK local)))
+               (Public (AK local))) ;
+     (CheckSig (sign (key (Public (AK initial))) (Private (CA oem)))
+               (Public (CA oem))) ;
+     (CheckSig (sign (TPM2_Attest (Private (AK local))) (Private (AK initial)))
+               (Public (AK initial))) ;
+(*7*)(MakeCert (Public (AK local)) (Private (CA owner))).
+
+Definition caOwnerFinal : state :=
+(*0*)(Union _ caOwnerIni
+(*5*)(send (sign lakCSR (Private (AK local))))) :
+(*7*)(sign (key (Public (AK local))) (Private (CA owner))). 
+
+Theorem CertLAK_spec :
+execute ownerIni ownerSteps ownerFinal /\
+In _ ownerFinal (sign lakCSR (Private (AK local))) /\
+execute (Union _ caOwnerIni (send (sign lakCSR (Private (AK local))))) caOwnerSteps caOwnerFinal.
+Proof.
+  repeat try split.
+  - apply correct_ownerFinal.
+  - unfold ownerFinal; unfold ownerIni; unfold lakCSR. apply Union_intror. apply In_singleton.
+  - unfold caOwnerFinal; unfold caOwnerIni; unfold caOwnerSteps; unfold lakCSR; simpl. 
+    repeat eapply E_Sequence.
+  -- apply E_CheckSigAK.
+  --- apply Union_intror. apply Union_intror. apply In_singleton.
+  --- apply Union_intror. apply Union_introl. apply Union_introl. apply Union_intror.
+      apply In_singleton.
+  -- apply E_CheckSigCA.
+  --- apply Union_intror. apply Union_introl. apply Union_introl. apply Union_introl.
+      apply Union_introl. apply Union_introl. apply Union_intror. apply In_singleton.
+  --- apply Union_introl. apply Union_intror. apply In_singleton.
+  -- apply E_CheckSigAK.
+  --- apply Union_intror. apply Union_introl. apply Union_introl. apply Union_introl.
+      apply Union_introl. apply Union_intror. apply Union_intror. apply In_singleton.
+  --- apply Union_intror. apply Union_introl. apply Union_introl. apply Union_introl.
+      apply Union_introl. apply Union_introl. apply Union_introl. apply In_singleton.
+  -- apply E_MakeCert.
+  --- apply Union_intror. apply Union_introl. apply Union_introl. apply Union_intror.
+      apply In_singleton.
+  --- apply Union_introl. apply Union_introl. apply In_singleton.
+Qed.
+
+
+
+
+
+
+
+
+
+
+
+(* OEM creation of IAK certificate based on EK certificate *)
+
+Definition oemIni : state :=
+(*0*)(Singleton _ (key (Private EK))) :
+     (sign (key (Public EK)) (Private (CA tm))).
+
+Definition iakCSR : message :=
+((sign (key (Public EK)) (Private (CA tm))),
+ (key (Public (AK initial))),
+ (key (Public (AK initial)))).
+
+Definition oemSteps1 : command :=
+(*1*)TPM2_Create (AK initial) ;
+(*2*)MakeCSR (sign (key (Public EK)) (Private (CA tm)))
+             (key (Public (AK initial))) (* TODO: replace with id*)
+             (Public (AK initial)) ;
+(*3*)TPM2_Sign iakCSR (Private (AK initial)).
+
+Definition oemMid : state :=
+(*0*)oemIni :
+(*1*)(key (Private (AK initial))) :
+     (key (Public (AK initial))) :
+(*2*)iakCSR :
+(*3*)(sign iakCSR (Private (AK initial))).
+
+
+Theorem correct_oemMid :
+execute oemIni oemSteps1 oemMid.
+Proof.
+  unfold oemMid; unfold oemIni; unfold oemSteps1; unfold iakCSR; simpl. 
+  repeat eapply E_Sequence. 
+  - apply E_Create.
+  - apply E_MakeCSR.
+  -- apply Union_introl. apply Union_introl. apply Union_intror. apply In_singleton.
+  -- apply Union_intror. apply In_singleton.
+  -- apply Union_intror. apply In_singleton.
+  - apply E_Sign.
+  -- apply Union_intror. apply In_singleton.
+  -- apply Union_introl. apply Union_introl. apply Union_intror. apply In_singleton.
+Qed.
+
+(*4*)(* send 3 *)
+
+Definition caOemIni : state :=
+(*0*)(Singleton _ (key (Private (CA oem)))) :
+     (key (Public (CA tm))).
+
+Definition caOemSteps1 : command :=
+(*5*)(CheckSig (sign iakCSR (Private (AK initial)))
+               (Public (AK initial))) ;
+     (CheckSig (sign (key (Public EK)) (Private (CA tm)))
+               (Public (CA tm))) ;
+(*6*)TPM2_MakeCredential (Public (AK initial)) (Public EK).
+
+Definition caOemMid : state :=
+(*0*)(Union _ caOemIni
+(*5*)(send (sign iakCSR (Private (AK initial))))) :
+(*6*)(encrypt (credential (key (Public (AK initial)))) (Public EK)).
+
+Theorem correct_caOemMid :
+execute oemIni oemSteps1 oemMid /\
+In _ oemMid (sign iakCSR (Private (AK initial))) /\
+execute (Union _ caOemIni (send (sign iakCSR (Private (AK initial))))) caOemSteps1 caOemMid.
+Proof.
+  repeat try split.
+  - apply correct_oemMid.
+  - unfold oemMid; unfold iakCSR. apply Union_intror. apply In_singleton.
+  - unfold caOemMid; unfold caOemIni; unfold caOemSteps1; unfold iakCSR; simpl. 
+    repeat eapply E_Sequence.
+  -- apply E_CheckSigAK.
+  --- apply Union_intror. apply Union_intror. apply In_singleton.
+  --- apply Union_intror. apply Union_introl. apply Union_introl. apply Union_intror.
+      apply In_singleton.
+  -- apply E_CheckSigCA.
+  --- apply Union_intror. apply Union_introl. apply Union_introl. apply Union_introl.
+      apply Union_introl. apply Union_introl. apply Union_intror. apply In_singleton.
+  --- apply Union_introl. apply Union_intror. apply In_singleton.
+  -- apply E_MakeCredential.
+  --- apply Union_intror. apply Union_introl. apply Union_introl. apply Union_intror.
+      apply In_singleton.
+  --- apply Union_intror. apply Union_introl. apply Union_introl. apply Union_introl.
+      apply Union_introl. apply Union_introl. apply Union_introl. apply In_singleton.
+Qed.
+
+(*7*)(* send 6*)
+
+Definition oemSteps2 : command :=
+(*8*)TPM2_ActivateCredential (encrypt (credential (key (Public (AK initial)))) (Public EK))
+                             (Private EK).
+
+Definition oemFinal : state :=
+(* *)(Union _ oemMid
+(*7*)(send (encrypt (credential (key (Public (AK initial)))) (Public EK)))) :
+(*8*)(credential (key (Public (AK initial)))).
+
+
+
+
+
+
+
+
+
+
+
+
+
+(* Owner creation of LAK certificate based on IAK certificate *)
 Section CertLAK.
 
 Inductive ak_val : Set :=
@@ -8,14 +396,14 @@ Inductive ak_val : Set :=
 | local : ak_val.
 
 Inductive ca_val : Set :=
-| tm : ca_val
-| oem : ca_val
+| tm : ca_val   (* tpm manufacturer *)
+| oem : ca_val  (* original equipment manufacturer *)
 | owner : ca_val.
 
 Inductive key_val : Set :=
-| EK : key_val 
-| AK : ak_val -> key_val
-| CA : ca_val -> key_val.
+| EK : key_val              (* endorsement key *)
+| AK : ak_val -> key_val    (* attestation key *)
+| CA : ca_val -> key_val.   (* certificate authority key *)
 
 Inductive keyType : Type := 
 | Private : key_val -> keyType
@@ -26,7 +414,7 @@ Inductive keyType : Type :=
 (* TODO: encrypt *)
 Inductive message : Type :=
 | key : keyType -> message
-| attest : keyType -> message
+| TPM2_Attest : keyType -> message
 | sign : message -> keyType -> message
 | pair : message -> message -> message.
 
@@ -44,7 +432,7 @@ Inductive command : Type :=
 | MakeCert : keyType -> keyType -> command
 | Sequence : command -> command -> command.
 
-Definition state := Ensemble message.
+Definition state := Ensemble message. (* ? should be decidable ? *)
 
 Notation "m1 , m2" := (pair m1 m2)  (at level 90, left associativity).
 Notation "c1 ; c2" := (Sequence c1 c2) (at level 90, left associativity).
@@ -56,22 +444,22 @@ Inductive execute : state -> command -> state -> Prop :=
 | E_Certify : forall st k k0,
     In _ st (key k) ->
     In _ st (key k0) ->
-    execute st (TPM2_Certify k k0) (st : (sign (attest k) k0))
+    execute st (TPM2_Certify k k0) (st : (sign (TPM2_Attest k) k0))
 | E_MakeCSR : forall st m1 m2 k,
     In _ st m1 ->
     In _ st m2 ->
     In _ st (key k) ->
     execute st (MakeCSR m1 m2 k) (st : m1 : m2 : (key k) : (m1, m2, (key k)))
 | E_Sign : forall st m k,
-    In _ st m -> (* ? *)
+    In _ st m ->
     In _ st (key k) ->
     execute st (TPM2_Sign m k) (st : (sign m k))
 | E_CheckSigAK : forall st m a,
-    In _ st m ->
+    In _ st m -> (* ? required ? *)
     In _ st (key (Public (AK a))) ->
     execute st (CheckSig (sign m (Private (AK a))) (Public (AK a))) st
 | E_CheckSigCA : forall st m c,
-    In _ st m ->
+    In _ st m -> (* ? required ? *)
     In _ st (key (Public (CA c))) ->
     execute st (CheckSig (sign m (Private (CA c))) (Public (CA c))) st
 | E_MakeCert : forall st k k0,
@@ -83,12 +471,54 @@ Inductive execute : state -> command -> state -> Prop :=
     execute st' c2 st'' ->
     execute st (Sequence c1 c2) st''.
 
+Inductive discoverable : message -> state -> Prop :=
+| D_key : forall k,
+    discoverable (key k) (Singleton _ (key k))
+| D_Attest : forall k,
+    discoverable (TPM2_Attest k) (Singleton _ (TPM2_Attest k))
+| D_sign : forall m k st, 
+    discoverable m st ->
+    discoverable (sign m k) (st : (sign m k))
+| D_pair : forall m1 m2 st1 st2,
+    discoverable m1 st1 ->
+    discoverable m2 st2 ->
+    discoverable (pair m1 m2) ((Union _ st1 st2) : (m1, m2)).
+
+(* when sending a message the recipient can discover everything in this result *)
 Fixpoint send (m : message) : state :=
 match m with
   | sign m0 k => (send m0) : (sign m0 k)
   | pair m1 m2 => (Union _ (send m1) (send m2)) : (m1, m2)
   | _ => Singleton _ m
 end.
+
+Theorem discoverableSend : forall m st,
+discoverable m st ->
+send m = st.
+Proof.
+  intros m st H; induction H; simpl; subst; reflexivity.
+Qed.
+
+Lemma sendDiscoverable' : forall m,
+discoverable m (send m).
+Proof.
+  intros m; induction m; simpl; constructor; assumption.
+Qed.
+
+Theorem sendDiscoverable : forall m st,
+send m = st -> 
+discoverable m st.
+Proof.
+  intros m st H; induction m; subst; apply sendDiscoverable'.
+Qed.
+
+Theorem iff_DiscoverableSend : forall m st,
+discoverable m st <-> send m = st.
+Proof.
+  split.
+  - apply discoverableSend.
+  - apply sendDiscoverable.
+Qed.
 
 Definition ownerIni : state :=
 (*0*)(Singleton _ (key (Private (AK initial)))) :
@@ -98,17 +528,17 @@ Definition ownerProtocol : command :=
 (*1*)TPM2_Create (AK local) ;
 (*2*)TPM2_Certify (Private (AK local)) (Private (AK initial)) ;
 (*3*)MakeCSR (sign (key (Public (AK initial))) (Private (CA oem))) 
-             (sign (attest (Private (AK local))) (Private (AK initial))) 
+             (sign (TPM2_Attest (Private (AK local))) (Private (AK initial))) 
              (Public (AK local)) ;
 (*4*)TPM2_Sign ((sign (key (Public (AK initial))) (Private (CA oem))), 
-                (sign (attest (Private (AK local))) (Private (AK initial))),
+                (sign (TPM2_Attest (Private (AK local))) (Private (AK initial))),
                 (key (Public (AK local)))) 
                (Private (AK local)).
 
 
 Definition csrLAK : message :=
   ((sign (key (Public (AK initial))) (Private (CA oem))),
-   (sign (attest (Private (AK local))) (Private (AK initial))),
+   (sign (TPM2_Attest (Private (AK local))) (Private (AK initial))),
    (key (Public (AK local)))).
 
 Definition ownerFinal : state :=
@@ -116,9 +546,9 @@ Definition ownerFinal : state :=
      (sign (key (Public (AK initial))) (Private (CA oem))) :
 (*1*)(key (Private (AK local))) :
      (key (Public (AK local))) :
-(*2*)(sign (attest (Private (AK local))) (Private (AK initial))) :
+(*2*)(sign (TPM2_Attest (Private (AK local))) (Private (AK initial))) :
 (*3*)(sign (key (Public (AK initial))) (Private (CA oem))) :
-     (sign (attest (Private (AK local))) (Private (AK initial))) :
+     (sign (TPM2_Attest (Private (AK local))) (Private (AK initial))) :
      (key (Public (AK local))) :
      csrLAK :
 (*4*)(sign csrLAK (Private (AK local))).
@@ -160,7 +590,7 @@ Definition caProtocol : command :=
                (Public (AK local))) ;
      (CheckSig (sign (key (Public (AK initial))) (Private (CA oem)))
                (Public (CA oem))) ;
-     (CheckSig (sign (attest (Private (AK local))) (Private (AK initial)))
+     (CheckSig (sign (TPM2_Attest (Private (AK local))) (Private (AK initial)))
                (Public (AK initial))) ;
 (*7*)(MakeCert (Public (AK local)) (Private (CA owner))).
 
